

# Ill-Typed Programs Don't Evaluate

Charlie Walpole

University of Bristol

6/7 November 2024

“Well-typed programs don't go wrong.” (Type Safety)

“Well-typed programs don't go wrong.” (Type Safety)

- ① Preservation
- ② Progress

“Well-typed programs don't go wrong.” (Type Safety)

- ① Preservation: “Evaluation preserves typing.”
- ② Progress: “Typed terms don't get stuck.”

“Well-typed programs don't go wrong.” (Type Safety)

- ① Preservation: “Evaluation preserves typing.”
- ② Progress: “Typed terms don't get stuck.”

$$\exists \tau. \vdash e : \tau \implies \exists \nu. e \Downarrow \nu$$

$$\exists \tau. \vdash e : \tau \implies \exists \nu. e \Downarrow \nu$$

$$\exists \tau. \vdash e : \tau \implies \exists \nu. e \Downarrow \nu$$

$(\forall \alpha) \quad \not\vdash \text{if } (\lambda x. x) \text{ True then } 1 \text{ else True} : \alpha$

$(\forall \alpha) \quad \not\vdash \text{if } (\lambda x. x) 1 \text{ then } 1 \text{ else } 1 : \alpha$

# Language

pre-terms	$e$	$::=$	$x$	variables
			$e_1\ e_2$	function application
			$\lambda x. e$	function abstraction
			$c(e_1, \dots, e_n)$	constructor application
			$\text{match } e_0 \text{ with } \{ \mid_{i=0}^n p_i \mapsto e_i \}$	pattern matching
types	$\tau$	$::=$	$\alpha$	type variables
			$\tau_1 \rightarrow \tau_2$	function arrow
			$\tau_1 + \tau_2$	sum types
			$c(\tau_1, \dots, \tau_n)$	constructor types
			Ok	top-type



# Language

pre-terms	$e ::=$	$x$	variables
		$e_1\ e_2$	function application
		$\lambda x. e$	function abstraction
		$c(e_1, \dots, e_n)$	constructor application
		$\text{match } e_0 \text{ with } \{ \mid_{i=0}^n p_i \mapsto e_i \}$	pattern matching
types	$\tau ::=$	$\alpha$	type variables
		$\tau_1 \rightarrow \tau_2$	function arrow
		$\tau_1 + \tau_2$	sum types
		$c(\tau_1, \dots, \tau_n)$	constructor types
		Ok	top-type

Language:

$$e := \lambda x. e \mid e_1 \ e_2 \mid x \mid c(e_1, \dots, e_n) \mid \text{match } e_0 \text{ with } \{ \mid_{i=1}^n p_i \mapsto e_i \}$$

Types:

$$\tau := \alpha \mid \tau_1 \rightarrow \tau_2 \mid \tau_1 + \tau_2 \mid c(\tau_1, \dots, \tau_n) \mid \text{Ok}$$

# Constructors - Terms & Types

zero :: zero

# Constructors - Terms & Types

```
zero    :: zero
succ(zero) :: succ(zero)
```

# Constructors - Terms & Types

zero	::	zero
succ(zero)	::	succ(zero)
succ(zero)	::	succ(Nat)
succ(zero)	::	Nat

# Constructors - Terms & Types

$$\begin{aligned} &\vdash \text{zero} : \text{zero} \\ &\vdash \text{succ}(\text{zero}) : \text{succ}(\text{zero}) \\ &\vdash \text{succ}(\text{zero}) : \text{succ}(\text{Nat}) \\ &\quad \vdash \text{succ}(\text{zero}) : \text{Nat} \end{aligned}$$

# Match Expressions

match  $e_0$  with  $\{ \mid_{i=1}^n p_i \mapsto e_i \}$

# Match Expressions

match  $e_0$  with  $\{ \mid_{i=1}^n p_i \mapsto e_i \}$

match  $\text{succ}(\text{zero})$  with  $\{ \mid \text{zero} \mapsto \text{zero}$   
 $\mid \text{succ}(n) \mapsto n \}$



$$(\forall \tau) \vdash e : \tau \implies \vdash e : \text{Ok}$$

$\neg(\vdash \text{if } (\lambda x. x) 1 \text{ then } 1 \text{ else } 1 : \text{Ok})$

# Typing Judgements

The typing judgement takes the form of:

$$x_1 : A_1, \dots, x_n : A_n \vdash e : B$$

# Typing Judgements

The typing judgement takes the form of:

$$x_1 : A_1, \dots, x_n : A_n \vdash e : B$$

We can intuitively read this as:

$$x_1 \in A_1 \wedge \dots \wedge x_n \in A_n \Rightarrow e \in B$$

# Typing Judgements

The typing judgement takes the form of:

$$x_1 : A_1, \dots, x_n : A_n \vdash e : B$$

We can intuitively read this as:

$$x_1 \in A_1 \wedge \dots \wedge x_n \in A_n \Rightarrow e \in B$$

$$\neg(x_1 : A_1 \vdash e : B) \Longrightarrow ???$$

$$\neg(x_1 \in A_1 \Rightarrow e \in B) \Longrightarrow x_1 \in A_1 \wedge \neg(e \in B)$$

We can define an operation,  $\llbracket \cdot \rrbracket$ , for both terms and types.  
Intuitively,  $e \Downarrow \nu \implies \nu \in \llbracket e \rrbracket$ .

We can define an operation,  $\llbracket \cdot \rrbracket$ , for both terms and types.

Intuitively,  $e \Downarrow \nu \implies \nu \in \llbracket e \rrbracket$ .

Term semantics:

$$\llbracket \text{zero} \rrbracket = \{0\} \subseteq \mathbb{Z}$$

$$\llbracket \text{zero} + \text{succ}(\text{zero}) \rrbracket = \{1\}$$

Type Semantics:

$$\begin{aligned}\llbracket \text{Nat} \rrbracket &:= \mathbb{Z} \\ \llbracket \tau_1 + \tau_2 \rrbracket &:= \llbracket \tau_1 \rrbracket \cup \llbracket \tau_2 \rrbracket\end{aligned}$$



# Denotational Semantics - (Partial) Definition

Type Semantics:

$$\begin{aligned}\llbracket \text{Nat} \rrbracket &:= \mathbb{Z} \\ \llbracket \tau_1 + \tau_2 \rrbracket &:= \llbracket \tau_1 \rrbracket \cup \llbracket \tau_2 \rrbracket \\ \llbracket \text{Ok} \rrbracket &:= \mathcal{U}\end{aligned}$$

Type Semantics:

$$\begin{aligned}\llbracket \text{Nat} \rrbracket &:= \mathbb{Z} \\ \llbracket \tau_1 + \tau_2 \rrbracket &:= \llbracket \tau_1 \rrbracket \cup \llbracket \tau_2 \rrbracket \\ \llbracket \text{Ok} \rrbracket &:= \mathcal{U} = \bigcup_{\tau} \llbracket \tau \rrbracket\end{aligned}$$

$$\llbracket \tau_1 \rightarrow \tau_2 \rrbracket := \{f \mid f : \mathcal{U} \rightarrow \mathcal{U}, x \in \llbracket \tau_1 \rrbracket \implies f(x) \in \llbracket \tau_2 \rrbracket\}$$

# Denotational Semantics - (Partial) Definition

$$\llbracket \tau_1 \rightarrow \tau_2 \rrbracket := \{f \mid f : \mathcal{U} \rightarrow \mathcal{U}, x \in \llbracket \tau_1 \rrbracket \implies f(x) \in \llbracket \tau_2 \rrbracket\} \\ \neq \llbracket \tau_1 \rrbracket \rightarrow \llbracket \tau_2 \rrbracket$$

# Logical Typing Judgements

Now, we can write ‘the meaning’ of a typing judgment:

$$x_1 : A_1, \dots, x_n : A_n \vdash e : B$$

As a logical statement:

$$\llbracket x_1 \rrbracket \subseteq \llbracket A_1 \rrbracket \wedge \dots \wedge \llbracket x_n \rrbracket \subseteq \llbracket A_n \rrbracket \implies \llbracket e \rrbracket \subseteq \llbracket B \rrbracket$$

# Negation

Our goal:

$$\neg(\vdash \text{if } (\lambda x. x) 1 \text{ then } 1 \text{ else } 1 : \text{Ok})$$

# Negation

Our goal:

$$\neg(\vdash \text{if } (\lambda x. x) 1 \text{ then } 1 \text{ else } 1 : \text{Ok})$$

Negation fact:

$$(\neg A) \iff (A \implies \perp)$$

# Negation

Our goal:

$$\neg(\vdash \text{if } (\lambda x. x) \ 1 \text{ then } 1 \text{ else } 1 : \text{Ok})$$

Negation fact:

$$(\neg A) \iff (A \implies \perp)$$

Thus:

$$\begin{aligned} \neg(\vdash \text{if } (\lambda x. x) \ 1 \text{ then } 1 \text{ else } 1 : \text{Ok}) &\iff \neg(\top \implies \llbracket \text{if } (\lambda x. x) \ 1 \text{ then } 1 \text{ else } 1 \rrbracket \subseteq \llbracket \text{Ok} \rrbracket) \\ &\iff ((\llbracket \text{if } 1 \text{ then } (\lambda x. x) \ 1 \text{ else } 1 \rrbracket \subseteq \llbracket \text{Ok} \rrbracket) \implies \perp) \end{aligned}$$



# Negation

Our goal:

$$\neg(\vdash \text{if } (\lambda x. x) \ 1 \text{ then } 1 \text{ else } 1 : \text{Ok})$$

Negation fact:

$$(\neg A) \iff (A \implies \perp)$$

Thus:

$$\begin{aligned} \neg(\vdash \text{if } (\lambda x. x) \ 1 \text{ then } 1 \text{ else } 1 : \text{Ok}) &\iff \neg(\top \implies \llbracket \text{if } (\lambda x. x) \ 1 \text{ then } 1 \text{ else } 1 \rrbracket \subseteq \llbracket \text{Ok} \rrbracket) \\ &\iff ((\llbracket \text{if } 1 \text{ then } (\lambda x. x) \ 1 \text{ else } 1 \rrbracket \subseteq \llbracket \text{Ok} \rrbracket) \implies \perp) \\ &\iff (\text{if } (\lambda x. x) \ 1 \text{ then } 1 \text{ else } 1 : \text{Ok} \vdash \perp) \end{aligned}$$

# Examining Typing Judgements

Take a general typing judgement:

$$x_1 : A_1, \dots, x_n : A_n \vdash e : B$$

Notable restrictions:

# Examining Typing Judgements

Take a general typing judgement:

$$x_1 : A_1, \dots, x_n : A_n \vdash e : B$$

Notable restrictions:

- 1 Only variable typings may appear in the context.

# Examining Typing Judgements

Take a general typing judgement:

$$x_1 : A_1, \dots, x_n : A_n \vdash e : B$$

Notable restrictions:

- 1 Only variable typings may appear in the context.
- 2 There must be exactly 1 typing as the conclusion.

# Examining Typing Judgements

Take a general typing judgement:

$$x_1 : A_1, \dots, x_n : A_n \vdash e : B$$

Notable restrictions:

- 1 Only variable typings may appear in the context.
- 2 There must be exactly 1 typing as the conclusion.

Lets relax these restrictions.

# Two Sides of Typing

Typing:

$$e_1 : A_1, \dots, e_n : A_n \vdash e'_1 : B_1, \dots, e'_m : B_m$$

# Two Sides of Typing

Typing:

$$e_1 : A_1, \dots, e_n : A_n \vdash e'_1 : B_1, \dots, e'_m : B_m$$

Logic:

$$\llbracket e_1 \rrbracket \subseteq \llbracket A_1 \rrbracket \wedge \dots \wedge \llbracket e_n \rrbracket \subseteq \llbracket A_n \rrbracket \implies \llbracket e'_1 \rrbracket \subseteq \llbracket B_1 \rrbracket \vee \dots \vee \llbracket e'_m \rrbracket \subseteq \llbracket B_m \rrbracket$$

# Two Sides of Typing

Typing:

$$e_1 : A_1, \dots, e_n : A_n \vdash e'_1 : B_1, \dots, e'_m : B_m$$

Logic:

$$\llbracket e_1 \rrbracket \subseteq \llbracket A_1 \rrbracket \wedge \dots \wedge \llbracket e_n \rrbracket \subseteq \llbracket A_n \rrbracket \implies \llbracket e'_1 \rrbracket \subseteq \llbracket B_1 \rrbracket \vee \dots \vee \llbracket e'_m \rrbracket \subseteq \llbracket B_m \rrbracket$$



# Sequent Calculus

$$P \wedge Q \wedge \top \iff P \wedge Q$$

$$P \wedge \top \iff P$$

$$(P_1 \wedge \dots \wedge P_n) \wedge \top \iff P_1 \wedge \dots \wedge P_n$$

# Sequent Calculus

$$P \wedge Q \wedge \top \iff P \wedge Q$$

$$P \wedge \top \iff P$$

$$(P_1 \wedge \dots \wedge P_n) \wedge \top \iff P_1 \wedge \dots \wedge P_n$$

$$P \vee Q \vee \perp \iff P \vee Q$$

$$P \vee \perp \iff P$$

$$(P_1 \vee \dots \vee P_n) \vee \perp \iff P_1 \vee \dots \vee P_n$$

$$e_1 : A_1, \dots, e_n : A_n \vdash$$

$$e_1 : A_1, \dots, e_n : A_n \vdash$$

$$\llbracket e_1 \rrbracket \subseteq \llbracket A_1 \rrbracket \wedge \dots \wedge \llbracket e_n \rrbracket \subseteq \llbracket A_n \rrbracket \implies \perp$$

$$e_1 : A_1, \dots, e_n : A_n \vdash \perp$$

$$\llbracket e_1 \rrbracket \subseteq \llbracket A_1 \rrbracket \wedge \dots \wedge \llbracket e_n \rrbracket \subseteq \llbracket A_n \rrbracket \implies \perp$$

Goal:

$$\neg(\vdash \text{if } (\lambda x. x) 1 \text{ then } 1 \text{ else } 1 : \text{Ok})$$

Translation:

$$\text{if } (\lambda x. x) 1 \text{ then } 1 \text{ else } 1 : \text{Ok} \vdash$$

# Examples of Note

①  $\vdash \text{map} : (\text{Nat} \geq 3 \rightarrow \text{Nat} \geq 8) \rightarrow [\text{Nat} \geq 3] \rightarrow [\text{Nat} \geq 8]$

# Examples of Note

- ①  $\vdash \text{map} : (\text{Nat} \geq 3 \rightarrow \text{Nat} \geq 8) \rightarrow [\text{Nat} \geq 3] \rightarrow [\text{Nat} \geq 8]$
- ②  $x + 1 : \text{Nat} \vdash (\lambda y. y) x : \text{Nat}$



# Examples of Note

- ①  $\vdash \text{map} : (\text{Nat} \geq 3 \rightarrow \text{Nat} \geq 8) \rightarrow [\text{Nat} \geq 3] \rightarrow [\text{Nat} \geq 8]$
- ②  $x + 1 : \text{Nat} \vdash (\lambda y. y) x : \text{Nat}$
- ③  $\text{Nil} : \text{Nat} \vdash$

# Examples of Note

- ①  $\vdash \text{map} : (\text{Nat} \geq 3 \rightarrow \text{Nat} \geq 8) \rightarrow [\text{Nat} \geq 3] \rightarrow [\text{Nat} \geq 8]$
- ②  $x + 1 : \text{Nat} \vdash (\lambda y. y) x : \text{Nat}$
- ③  $\text{Nil} : \text{Nat} \vdash$
- ④  $1 + \text{Nil} : \text{Ok} \vdash$

# Examples of Note

- ①  $\vdash \text{map} : (\text{Nat} \geq 3 \rightarrow \text{Nat} \geq 8) \rightarrow [\text{Nat} \geq 3] \rightarrow [\text{Nat} \geq 8]$
- ②  $x + 1 : \text{Nat} \vdash (\lambda y. y) x : \text{Nat}$
- ③  $\text{Nil} : \text{Nat} \vdash$
- ④  $1 + \text{Nil} : \text{Ok} \vdash$
- ⑤  $\text{match Nil with } \{\text{Cons}(y, ys) \mapsto y\} : \text{Ok} \vdash$

# Examples of Note

- ①  $\vdash \text{map} : (\text{Nat} \geq 3 \rightarrow \text{Nat} \geq 8) \rightarrow [\text{Nat} \geq 3] \rightarrow [\text{Nat} \geq 8]$
- ②  $x + 1 : \text{Nat} \vdash (\lambda y. y) x : \text{Nat}$
- ③  $\text{Nil} : \text{Nat} \vdash$
- ④  $1 + \text{Nil} : \text{Ok} \vdash$
- ⑤  $\text{match Nil with } \{\text{Cons}(y, ys) \mapsto y\} : \text{Ok} \vdash$

How are these derived/proven?

# Deriving Typing Rules

Let's derive a typing rule for  $(e_1, e_2) : A_1 \times A_2 \vdash$ :

# Deriving Typing Rules

Let's derive a typing rule for  $(e_1, e_2) : A_1 \times A_2 \vdash$ :

$$(e_1, e_2) : A_1 \times A_2 \vdash$$

# Deriving Typing Rules

Let's derive a typing rule for  $(e_1, e_2) : A_1 \times A_2 \vdash$ :

$$\begin{aligned} & (e_1, e_2) : A_1 \times A_2 \vdash \\ \iff & \neg(\llbracket (e_1, e_2) \rrbracket \subseteq \llbracket A_1 \times A_2 \rrbracket) \end{aligned}$$

# Deriving Typing Rules

Let's derive a typing rule for  $(e_1, e_2) : A_1 \times A_2 \vdash$ :

$$\begin{aligned} & (e_1, e_2) : A_1 \times A_2 \vdash \\ \iff & \neg(\llbracket (e_1, e_2) \rrbracket \subseteq \llbracket A_1 \times A_2 \rrbracket) \\ \iff & \neg(\forall p. p \in \llbracket (e_1, e_2) \rrbracket \implies p \in \llbracket A_1 \times A_2 \rrbracket) \end{aligned}$$



# Deriving Typing Rules

Let's derive a typing rule for  $(e_1, e_2) : A_1 \times A_2 \vdash$ :

$$(e_1, e_2) : A_1 \times A_2 \vdash$$

$$\iff \neg(\llbracket (e_1, e_2) \rrbracket \subseteq \llbracket A_1 \times A_2 \rrbracket)$$

$$\iff \neg(\forall p. p \in \llbracket (e_1, e_2) \rrbracket \implies p \in \llbracket A_1 \times A_2 \rrbracket)$$

$$\iff \neg(\forall x, y. (x, y) \in \llbracket e_1 \rrbracket \times \llbracket e_2 \rrbracket \implies (x, y) \in \llbracket A_1 \rrbracket \times \llbracket A_2 \rrbracket)$$

# Deriving Typing Rules

Let's derive a typing rule for  $(e_1, e_2) : A_1 \times A_2 \vdash$ :

$$\begin{aligned} & (e_1, e_2) : A_1 \times A_2 \vdash \\ \iff & \neg(\llbracket (e_1, e_2) \rrbracket \subseteq \llbracket A_1 \times A_2 \rrbracket) \\ \iff & \neg(\forall p. p \in \llbracket (e_1, e_2) \rrbracket \implies p \in \llbracket A_1 \times A_2 \rrbracket) \\ \iff & \neg(\forall x, y. (x, y) \in \llbracket e_1 \rrbracket \times \llbracket e_2 \rrbracket \implies (x, y) \in \llbracket A_1 \rrbracket \times \llbracket A_2 \rrbracket) \\ \iff & \neg(\forall x, y. x \in \llbracket e_1 \rrbracket \wedge y \in \llbracket e_2 \rrbracket \implies x \in \llbracket A_1 \rrbracket \wedge y \in \llbracket A_2 \rrbracket) \end{aligned}$$

# Deriving Typing Rules

Let's derive a typing rule for  $(e_1, e_2) : A_1 \times A_2 \vdash$ :

$$\begin{aligned} & (e_1, e_2) : A_1 \times A_2 \vdash \\ \iff & \neg(\llbracket (e_1, e_2) \rrbracket \subseteq \llbracket A_1 \times A_2 \rrbracket) \\ \iff & \neg(\forall p. p \in \llbracket (e_1, e_2) \rrbracket \implies p \in \llbracket A_1 \times A_2 \rrbracket) \\ \iff & \neg(\forall x, y. (x, y) \in \llbracket e_1 \rrbracket \times \llbracket e_2 \rrbracket \implies (x, y) \in \llbracket A_1 \rrbracket \times \llbracket A_2 \rrbracket) \\ \iff & \neg(\forall x, y. x \in \llbracket e_1 \rrbracket \wedge y \in \llbracket e_2 \rrbracket \implies x \in \llbracket A_1 \rrbracket \wedge y \in \llbracket A_2 \rrbracket) \\ \iff & \exists x, y. x \in \llbracket e_1 \rrbracket \wedge y \in \llbracket e_2 \rrbracket \wedge \neg(x \in \llbracket A_1 \rrbracket \wedge y \in \llbracket A_2 \rrbracket) \end{aligned}$$

# Deriving Typing Rules

Let's derive a typing rule for  $(e_1, e_2) : A_1 \times A_2 \vdash$ :

$$\begin{aligned} & (e_1, e_2) : A_1 \times A_2 \vdash \\ \iff & \neg(\llbracket (e_1, e_2) \rrbracket \subseteq \llbracket A_1 \times A_2 \rrbracket) \\ \iff & \neg(\forall p. p \in \llbracket (e_1, e_2) \rrbracket \implies p \in \llbracket A_1 \times A_2 \rrbracket) \\ \iff & \neg(\forall x, y. (x, y) \in \llbracket e_1 \rrbracket \times \llbracket e_2 \rrbracket \implies (x, y) \in \llbracket A_1 \rrbracket \times \llbracket A_2 \rrbracket) \\ \iff & \neg(\forall x, y. x \in \llbracket e_1 \rrbracket \wedge y \in \llbracket e_2 \rrbracket \implies x \in \llbracket A_1 \rrbracket \wedge y \in \llbracket A_2 \rrbracket) \\ \iff & \exists x, y. x \in \llbracket e_1 \rrbracket \wedge y \in \llbracket e_2 \rrbracket \wedge \neg(x \in \llbracket A_1 \rrbracket \wedge y \in \llbracket A_2 \rrbracket) \\ \iff & \exists x, y. x \in \llbracket e_1 \rrbracket \wedge y \in \llbracket e_2 \rrbracket \wedge (x \notin \llbracket A_1 \rrbracket \vee y \notin \llbracket A_2 \rrbracket) \end{aligned}$$

# Deriving Typing Rules

Let's derive a typing rule for  $(e_1, e_2) : A_1 \times A_2 \vdash$ :

$$\begin{aligned} & (e_1, e_2) : A_1 \times A_2 \vdash \\ \iff & \neg(\llbracket (e_1, e_2) \rrbracket \subseteq \llbracket A_1 \times A_2 \rrbracket) \\ \iff & \neg(\forall p. p \in \llbracket (e_1, e_2) \rrbracket \implies p \in \llbracket A_1 \times A_2 \rrbracket) \\ \iff & \neg(\forall x, y. (x, y) \in \llbracket e_1 \rrbracket \times \llbracket e_2 \rrbracket \implies (x, y) \in \llbracket A_1 \rrbracket \times \llbracket A_2 \rrbracket) \\ \iff & \neg(\forall x, y. x \in \llbracket e_1 \rrbracket \wedge y \in \llbracket e_2 \rrbracket \implies x \in \llbracket A_1 \rrbracket \wedge y \in \llbracket A_2 \rrbracket) \\ \iff & \exists x, y. x \in \llbracket e_1 \rrbracket \wedge y \in \llbracket e_2 \rrbracket \wedge \neg(x \in \llbracket A_1 \rrbracket \wedge y \in \llbracket A_2 \rrbracket) \\ \iff & \exists x, y. x \in \llbracket e_1 \rrbracket \wedge y \in \llbracket e_2 \rrbracket \wedge (x \notin \llbracket A_1 \rrbracket \vee y \notin \llbracket A_2 \rrbracket) \\ \iff & \exists i. \exists x. x \in \llbracket e_i \rrbracket \wedge x \notin \llbracket A_i \rrbracket \end{aligned}$$

# Deriving Typing Rules

Let's derive a typing rule for  $(e_1, e_2) : A_1 \times A_2 \vdash$ :

$$\begin{aligned} & (e_1, e_2) : A_1 \times A_2 \vdash \\ \iff & \neg(\llbracket (e_1, e_2) \rrbracket \subseteq \llbracket A_1 \times A_2 \rrbracket) \\ \iff & \neg(\forall p. p \in \llbracket (e_1, e_2) \rrbracket \implies p \in \llbracket A_1 \times A_2 \rrbracket) \\ \iff & \neg(\forall x, y. (x, y) \in \llbracket e_1 \rrbracket \times \llbracket e_2 \rrbracket \implies (x, y) \in \llbracket A_1 \rrbracket \times \llbracket A_2 \rrbracket) \\ \iff & \neg(\forall x, y. x \in \llbracket e_1 \rrbracket \wedge y \in \llbracket e_2 \rrbracket \implies x \in \llbracket A_1 \rrbracket \wedge y \in \llbracket A_2 \rrbracket) \\ \iff & \exists x, y. x \in \llbracket e_1 \rrbracket \wedge y \in \llbracket e_2 \rrbracket \wedge \neg(x \in \llbracket A_1 \rrbracket \wedge y \in \llbracket A_2 \rrbracket) \\ \iff & \exists x, y. x \in \llbracket e_1 \rrbracket \wedge y \in \llbracket e_2 \rrbracket \wedge (x \notin \llbracket A_1 \rrbracket \vee y \notin \llbracket A_2 \rrbracket) \\ \iff & \exists i. \exists x. x \in \llbracket e_i \rrbracket \wedge x \notin \llbracket A_i \rrbracket \\ \iff & \exists i. \neg(\forall x. x \in \llbracket e_i \rrbracket \implies x \in \llbracket A_i \rrbracket) \end{aligned}$$

# Deriving Typing Rules

Let's derive a typing rule for  $(e_1, e_2) : A_1 \times A_2 \vdash$ :

$$\begin{aligned} & (e_1, e_2) : A_1 \times A_2 \vdash \\ \iff & \neg(\llbracket (e_1, e_2) \rrbracket \subseteq \llbracket A_1 \times A_2 \rrbracket) \\ \iff & \neg(\forall p. p \in \llbracket (e_1, e_2) \rrbracket \implies p \in \llbracket A_1 \times A_2 \rrbracket) \\ \iff & \neg(\forall x, y. (x, y) \in \llbracket e_1 \rrbracket \times \llbracket e_2 \rrbracket \implies (x, y) \in \llbracket A_1 \rrbracket \times \llbracket A_2 \rrbracket) \\ \iff & \neg(\forall x, y. x \in \llbracket e_1 \rrbracket \wedge y \in \llbracket e_2 \rrbracket \implies x \in \llbracket A_1 \rrbracket \wedge y \in \llbracket A_2 \rrbracket) \\ \iff & \exists x, y. x \in \llbracket e_1 \rrbracket \wedge y \in \llbracket e_2 \rrbracket \wedge \neg(x \in \llbracket A_1 \rrbracket \wedge y \in \llbracket A_2 \rrbracket) \\ \iff & \exists x, y. x \in \llbracket e_1 \rrbracket \wedge y \in \llbracket e_2 \rrbracket \wedge (x \notin \llbracket A_1 \rrbracket \vee y \notin \llbracket A_2 \rrbracket) \\ \iff & \exists i. \exists x. x \in \llbracket e_i \rrbracket \wedge x \notin \llbracket A_i \rrbracket \\ \iff & \exists i. \neg(\forall x. x \in \llbracket e_i \rrbracket \implies x \in \llbracket A_i \rrbracket) \\ \iff & \exists i. \neg(\llbracket e_i \rrbracket \subseteq \llbracket A_i \rrbracket) \end{aligned}$$

# Deriving Typing Rules

Let's derive a typing rule for  $(e_1, e_2) : A_1 \times A_2 \vdash$ :

$$\begin{aligned} & (e_1, e_2) : A_1 \times A_2 \vdash \\ \iff & \neg(\llbracket (e_1, e_2) \rrbracket \subseteq \llbracket A_1 \times A_2 \rrbracket) \\ \iff & \neg(\forall p. p \in \llbracket (e_1, e_2) \rrbracket \implies p \in \llbracket A_1 \times A_2 \rrbracket) \\ \iff & \neg(\forall x, y. (x, y) \in \llbracket e_1 \rrbracket \times \llbracket e_2 \rrbracket \implies (x, y) \in \llbracket A_1 \rrbracket \times \llbracket A_2 \rrbracket) \\ \iff & \neg(\forall x, y. x \in \llbracket e_1 \rrbracket \wedge y \in \llbracket e_2 \rrbracket \implies x \in \llbracket A_1 \rrbracket \wedge y \in \llbracket A_2 \rrbracket) \\ \iff & \exists x, y. x \in \llbracket e_1 \rrbracket \wedge y \in \llbracket e_2 \rrbracket \wedge \neg(x \in \llbracket A_1 \rrbracket \wedge y \in \llbracket A_2 \rrbracket) \\ \iff & \exists x, y. x \in \llbracket e_1 \rrbracket \wedge y \in \llbracket e_2 \rrbracket \wedge (x \notin \llbracket A_1 \rrbracket \vee y \notin \llbracket A_2 \rrbracket) \\ \iff & \exists i. \exists x. x \in \llbracket e_i \rrbracket \wedge x \notin \llbracket A_i \rrbracket \\ \iff & \exists i. \neg(\forall x. x \in \llbracket e_i \rrbracket \implies x \in \llbracket A_i \rrbracket) \\ \iff & \exists i. \neg(\llbracket e_i \rrbracket \subseteq \llbracket A_i \rrbracket) \\ \iff & \exists i. e_i : A_i \vdash \end{aligned}$$



# Deriving Typing Rules

Let's derive a typing rule for  $(e_1, e_2) : A_1 \times A_2 \vdash$ :

$$\begin{array}{l} (e_1, e_2) : A_1 \times A_2 \vdash \\ \iff \exists i. e_i : A_i \vdash \end{array}$$

# Deriving Typing Rules

Let's derive a typing rule for  $(e_1, e_2) : A_1 \times A_2 \vdash$ :

$$\begin{aligned} & (e_1, e_2) : A_1 \times A_2 \vdash \\ \iff & \exists i. e_i : A_i \vdash \end{aligned}$$

$$\text{(PairL)} \frac{(\exists i.) \Gamma, e_i : A_i \vdash \Delta}{\Gamma, (e_1, e_2) : A_1 \times A_2 \vdash \Delta}$$

# Deriving Typing Rules

Let's derive a typing rule for  $(e_1, e_2) : A_1 \times A_2 \vdash$ :

$$\begin{aligned} & (e_1, e_2) : A_1 \times A_2 \vdash \\ \iff & \exists i. e_i : A_i \vdash \end{aligned}$$

$$\begin{array}{c} \text{(PairL)} \frac{(\exists i.) \Gamma, e_i : A_i \vdash \Delta}{\Gamma, (e_1, e_2) : A_1 \times A_2 \vdash \Delta} \quad \text{(PairR)} \frac{(\forall i.) \Gamma \vdash e_i : A_i, \Delta}{\Gamma \vdash (e_1, e_2) : A_1 \times A_2, \Delta} \end{array}$$

# Deriving Typing Rules

So we have derived a new typing rule:

$$\text{(PairL)} \frac{(\exists i.) \Gamma, e_i : A_i \vdash \Delta}{\Gamma, (e_1, e_2) : A_1 \times A_2 \vdash \Delta} \quad \text{(PairR)} \frac{(\forall i.) \Gamma \vdash e_i : A_i, \Delta}{\Gamma \vdash (e_1, e_2) : A_1 \times A_2, \Delta}$$

And the key point in its derivation is:

$$x \notin \llbracket A_1 \times A_2 \rrbracket \iff (x \notin \llbracket A_1 \rrbracket \vee x \notin \llbracket A_2 \rrbracket)$$

Alternatively:

$$\llbracket A_1 \times A_2 \rrbracket^c = \llbracket A_1 \rrbracket^c \cup \llbracket A_2 \rrbracket^c$$

# Deriving Typing Rules - If

$$\text{(IfR)} \frac{\Gamma \vdash e_0 : \text{Bool} \quad \Gamma \vdash e_1 : \tau \quad \Gamma \vdash e_2 : \tau}{\Gamma \vdash \text{if } e_0 \text{ then } e_1 \text{ else } e_2 : \tau}$$

$$\frac{?}{\text{if } e_0 \text{ then } e_1 \text{ else } e_2 : \tau \vdash}$$

# Deriving Typing Rules - App

$$\text{(AppR)} \frac{\Gamma \vdash e_0 : \tau_1 \rightarrow \tau_2 \quad \Gamma \vdash e_1 : \tau_1}{\Gamma \vdash e_0 \ e_1 : \tau_2}$$

$$\frac{?}{e_0 \ e_1 : \tau_2 \vdash}$$

# Why does AppR work?

To prove the (AppR) rule correct, we show:

Given:

$$\Gamma \vdash e_0 : \tau_1 \rightarrow \tau_2$$

$$\Gamma \vdash e_1 : \tau_1$$

We want to show:

$$\Gamma \vdash (e_0 \ e_1) : \tau_2$$

# Why does AppR work?

To prove the (AppR) rule correct, we show:

Given:

$$\begin{aligned} \llbracket \Gamma \rrbracket &\Longrightarrow \llbracket e_0 \rrbracket \subseteq \llbracket \tau_1 \rightarrow \tau_2 \rrbracket \\ \llbracket \Gamma \rrbracket &\Longrightarrow \llbracket e_1 \rrbracket \subseteq \llbracket \tau_1 \rrbracket \end{aligned}$$

We want to show:

$$\llbracket \Gamma \rrbracket \Longrightarrow \llbracket e_0 \ e_1 \rrbracket \subseteq \llbracket \tau_2 \rrbracket$$



# Why does AppR work?

To prove the (AppR) rule correct, we show:

Given:

$$\begin{aligned} \llbracket e_0 \rrbracket &\subseteq \llbracket \tau_1 \rightarrow \tau_2 \rrbracket \\ \llbracket e_1 \rrbracket &\subseteq \llbracket \tau_1 \rrbracket \end{aligned}$$

We want to show:

$$\llbracket e_0 \ e_1 \rrbracket \subseteq \llbracket \tau_2 \rrbracket$$

# Why does AppR work?

To prove the (AppR) rule correct, we show:

Given:

$$\begin{aligned} \llbracket e_0 \rrbracket &\subseteq \{f \mid f : \mathcal{U} \rightarrow \mathcal{U}, x \in \llbracket \tau_1 \rrbracket \implies f(x) \in \llbracket \tau_2 \rrbracket\} \\ \llbracket e_1 \rrbracket &\subseteq \llbracket \tau_1 \rrbracket \end{aligned}$$

We want to show:

$$\llbracket e_0 \ e_1 \rrbracket \subseteq \llbracket \tau_2 \rrbracket$$

# Why does AppR work?

To prove the (AppR) rule correct, we show:

Given:

$$\begin{aligned} \llbracket e_0 \rrbracket &\subseteq \{f \mid f : \mathcal{U} \rightarrow \mathcal{U}, x \in \llbracket \tau_1 \rrbracket \implies f(x) \in \llbracket \tau_2 \rrbracket\} \\ \llbracket e_1 \rrbracket &\subseteq \llbracket \tau_1 \rrbracket \end{aligned}$$

We want to show:

$$\{f(x) \mid f \in \llbracket e_0 \rrbracket, x \in \llbracket e_1 \rrbracket\} \subseteq \llbracket \tau_2 \rrbracket$$

# Why doesn't this AppL work?

$$\frac{\Gamma \vdash e_0 : \tau_1 \rightarrow \tau_2 \quad \Gamma, e_1 : \tau_1 \vdash}{\Gamma, (e_0 \ e_1) : \tau_2 \vdash}$$

Given:

$$\begin{aligned} \llbracket e_0 \rrbracket \subseteq \{f \mid f : \mathcal{U} \rightarrow \mathcal{U}, x \in \llbracket \tau_1 \rrbracket \implies f(x) \in \llbracket \tau_2 \rrbracket\} \\ \neg(\llbracket e_1 \rrbracket \subseteq \llbracket \tau_1 \rrbracket) \end{aligned}$$

We want to show:

$$\neg(\{f(x) \mid f \in \llbracket e_0 \rrbracket, x \in \llbracket e_1 \rrbracket\} \subseteq \llbracket \tau_2 \rrbracket)$$

# What do we want?

$$\llbracket ? \rrbracket := \{f \mid f : \mathcal{U} \rightarrow \mathcal{U}, f(x) \in \llbracket \tau_2 \rrbracket \implies x \in \llbracket \tau_1 \rrbracket\}$$

# What do we want?

$$\llbracket \tau_1 \succ \tau_2 \rrbracket := \{f \mid f : \mathcal{U} \rightarrow \mathcal{U}, f(x) \in \llbracket \tau_2 \rrbracket \implies x \in \llbracket \tau_1 \rrbracket\}$$

$$A \succ B$$

“A only to B”

## Sufficiency

$$\frac{\Gamma, x : A \vdash e : B, \Delta}{\Gamma \vdash \lambda x. e : A \rightarrow B, \Delta} \text{ (AbsR)}$$

## Necessity

$$\text{ (AbnR) } \frac{\Gamma, e : B \vdash x : A, \Delta}{\Gamma \vdash \lambda x. e : A \rhd B, \Delta}$$



## Sufficiency

$$\frac{\Gamma, x : A \vdash e : B, \Delta}{\Gamma \vdash \lambda x. e : A \rightarrow B, \Delta} \text{ (AbsR)}$$

$\vdash \lambda x. 42 : \text{Nat} \rightarrow \text{Nat}$

## Necessity

$$\text{ (AbnR) } \frac{\Gamma, e : B \vdash x : A, \Delta}{\Gamma \vdash \lambda x. e : A \multimap B, \Delta}$$

## Sufficiency

$$\frac{\Gamma, x : A \vdash e : B, \Delta}{\Gamma \vdash \lambda x. e : A \rightarrow B, \Delta} \text{ (AbsR)}$$

$\vdash \lambda x. 42 : \text{Nat} \rightarrow \text{Nat}$

$\vdash \text{map } f : \text{Nil} \rightarrow \text{Nil}$

## Necessity

$$\text{ (AbnR) } \frac{\Gamma, e : B \vdash x : A, \Delta}{\Gamma \vdash \lambda x. e : A \multimap B, \Delta}$$

## Sufficiency

$$\frac{\Gamma, x : A \vdash e : B, \Delta}{\Gamma \vdash \lambda x. e : A \rightarrow B, \Delta} \text{ (AbsR)}$$

$\vdash \lambda x. 42 : \text{Nat} \rightarrow \text{Nat}$

$\vdash \text{map } f : \text{Nil} \rightarrow \text{Nil}$

$\vdash \text{map } f : \text{Nil} \rightarrow \text{List } \alpha$

## Necessity

$$\text{ (AbnR) } \frac{\Gamma, e : B \vdash x : A, \Delta}{\Gamma \vdash \lambda x. e : A \multimap B, \Delta}$$

## Sufficiency

$$\frac{\Gamma, x : A \vdash e : B, \Delta}{\Gamma \vdash \lambda x. e : A \rightarrow B, \Delta} \text{ (AbsR)}$$

$\vdash \lambda x. 42 : \text{Nat} \rightarrow \text{Nat}$

$\vdash \text{map } f : \text{Nil} \rightarrow \text{Nil}$

$\vdash \text{map } f : \text{Nil} \rightarrow \text{List } \alpha$

$\not\vdash \text{map } f : \text{List}(\alpha) \rightarrow \text{Nil}$

## Necessity

$$\text{ (AbnR) } \frac{\Gamma, e : B \vdash x : A, \Delta}{\Gamma \vdash \lambda x. e : A \multimap B, \Delta}$$

## Sufficiency

$$\frac{\Gamma, x : A \vdash e : B, \Delta}{\Gamma \vdash \lambda x. e : A \rightarrow B, \Delta} \text{ (AbsR)}$$

$\vdash \lambda x. 42 : \text{Nat} \rightarrow \text{Nat}$

$\vdash \text{map } f : \text{Nil} \rightarrow \text{Nil}$

$\vdash \text{map } f : \text{Nil} \rightarrow \text{List } \alpha$

$\not\vdash \text{map } f : \text{List}(\alpha) \rightarrow \text{Nil}$

## Necessity

$$\text{ (AbnR) } \frac{\Gamma, e : B \vdash x : A, \Delta}{\Gamma \vdash \lambda x. e : A \succ B, \Delta}$$

$\vdash \text{head} : \text{Cons}(\alpha, \text{Ok}) \succ \alpha$

## Sufficiency

$$\frac{\Gamma, x : A \vdash e : B, \Delta}{\Gamma \vdash \lambda x. e : A \rightarrow B, \Delta} \text{ (AbsR)}$$

$\vdash \lambda x. 42 : \text{Nat} \rightarrow \text{Nat}$

$\vdash \text{map } f : \text{Nil} \rightarrow \text{Nil}$

$\vdash \text{map } f : \text{Nil} \rightarrow \text{List } \alpha$

$\nvdash \text{map } f : \text{List}(\alpha) \rightarrow \text{Nil}$

## Necessity

$$\text{ (AbnR) } \frac{\Gamma, e : B \vdash x : A, \Delta}{\Gamma \vdash \lambda x. e : A \succ B, \Delta}$$

$\vdash \text{head} : \text{Cons}(\alpha, \text{Ok}) \succ \alpha$

$\vdash \text{map } f : \text{Nil} \succ \text{Nil}$

## Sufficiency

$$\frac{\Gamma, x : A \vdash e : B, \Delta}{\Gamma \vdash \lambda x. e : A \rightarrow B, \Delta} \text{ (AbsR)}$$

$\vdash \lambda x. 42 : \text{Nat} \rightarrow \text{Nat}$

$\vdash \text{map } f : \text{Nil} \rightarrow \text{Nil}$

$\vdash \text{map } f : \text{Nil} \rightarrow \text{List } \alpha$

$\not\vdash \text{map } f : \text{List}(\alpha) \rightarrow \text{Nil}$

## Necessity

$$\text{ (AbnR) } \frac{\Gamma, e : B \vdash x : A, \Delta}{\Gamma \vdash \lambda x. e : A \succ B, \Delta}$$

$\vdash \text{head} : \text{Cons}(\alpha, \text{Ok}) \succ \alpha$

$\vdash \text{map } f : \text{Nil} \succ \text{Nil}$

$\vdash \text{map } f : \text{List } \alpha \succ \text{Nil}$

## Sufficiency

$$\frac{\Gamma, x : A \vdash e : B, \Delta}{\Gamma \vdash \lambda x. e : A \rightarrow B, \Delta} \text{ (AbsR)}$$

$\vdash \lambda x. 42 : \text{Nat} \rightarrow \text{Nat}$

$\vdash \text{map } f : \text{Nil} \rightarrow \text{Nil}$

$\vdash \text{map } f : \text{Nil} \rightarrow \text{List } \alpha$

$\nvdash \text{map } f : \text{List}(\alpha) \rightarrow \text{Nil}$

## Necessity

$$\text{ (AbnR)} \frac{\Gamma, e : B \vdash x : A, \Delta}{\Gamma \vdash \lambda x. e : A \succ B, \Delta}$$

$\vdash \text{head} : \text{Cons}(\alpha, \text{Ok}) \succ \alpha$

$\vdash \text{map } f : \text{Nil} \succ \text{Nil}$

$\vdash \text{map } f : \text{List } \alpha \succ \text{Nil}$

$\nvdash \lambda x. 42 : \text{Nat} \succ \text{Nat}$



# Application on the Left

Now we have:

$$(\text{AppL}) \frac{\Gamma \vdash e_1 : A \multimap B, \Delta \quad \Gamma, e_2 : A \vdash \Delta}{\Gamma, e_1 e_2 : B \vdash \Delta}$$

# Application on the Left

Now we have:

$$(\text{AppL}) \frac{\Gamma \vdash e_1 : A \multimap B, \Delta \quad \Gamma, e_2 : A \vdash \Delta}{\Gamma, e_1 e_2 : B \vdash \Delta}$$

$$\begin{array}{c} (\text{AppL}) \frac{\vdash \lambda x. x : \text{Bool} \multimap \text{Bool} \quad 1 : \text{Bool} \vdash}{(\lambda x. x) 1 : \text{Bool} \vdash} \\ (\text{IfL1}) \frac{}{\text{if } (\lambda x. x) 1 \text{ then } 1 \text{ else } 1 : \text{Ok} \vdash} \end{array}$$

“(if (λx. x) 1 then 1 else 1) does not evaluate (reach a value)”

$$\vdash e : \text{Ok}$$

“Well-typed programs don’t go wrong.”

No execution of a well-typed program can crash.

$$e : \text{Ok} \vdash$$

“Ill-typed programs don’t evaluate.”

No execution of an ill-typed program can reach a value.